pcuic/theories/PCUICCumulativity.v
@@ -55,7 +55,6 @@ Proof.
 
   - apply Nat.eqb_refl.
   - apply eq_string_refl.
-  - apply Nat.eqb_refl.
   - rewrite /eq_evar eq_nat_refl.
     simpl. induction H0; simpl; auto. now rewrite p IHAll.
   - apply eq_universe_refl.
